Use more semantic style of coinduction

trunk/coq/playground/himp/simple_proofs.v
@@ -6,50 +6,160 @@ Open Scope string_scope.
 
 Require Import domains.
 Require Import kstyle.
-Require Import evaluator.
+Require Import coinduction.
 
 Coercion EVar : string >-> Exp.
 Coercion ECon : Z >-> Exp.
 
 Open Scope Z_scope.
+
+(* One thing to try is defining a simple wrapper to turn a parameterized rule
+   into a relation, see if we can get it automatically *)
+
+Ltac kequiv_tac := repeat (apply conj);[reflexivity|simpl;equate_maps ..].
+Ltac kstep_tac := econstructor(reflexivity || (simpl;find_map_entry)).
+
+(*
+(* Either solve immediately by using the circularity,
+   or bail out for manual intervention if the
+   circularity matches structurally *)
+Ltac use_circ circ :=
+  solve[eapply circ;
+  try (match goal with [|- _ ~= _] => equate_maps;reflexivity end);
+  instantiate;  omega]
+  || (eapply circ;fail 1).
+
+Ltac run := repeat (step_rule || split_if || finish).
+Ltac run_circ circ := repeat (use_circ circ || (step_rule || split_if || finish)).
+
+Ltac tstep := refine (Delay (itstep _ _ _ _));[econstructor (solve[reflexivity || find_map_entry])|].
+Ltac tsplit_if := cbv beta; (* reduce redexes left from plugging *)
+  match goal with
+      | [|- tsteps (KCfg (kra (KStmt (SIf (BCon (?x <=? ?y)%Z) _ _)) _) _ _ _) _] =>
+        pose proof (Zle_cases x y); destruct (x <=? y)%Z
+  end.
+ *)
+
+Notation basic_goal rel :=
+  (forall env,
+  rel (KCfg (kra (SAssign "x" (EPlus "x" "y")) nil)
+            (env :* "x" |-> 12%Z :* "y" |-> 13%Z) mapEmpty mapEmpty)
+      (kequiv (KCfg nil (env :* "x" |-> 25%Z :* "y" |-> 13%Z) mapEmpty mapEmpty))).
+(* Very basic example, no heaps or labels, and even using derived rules *)
+Lemma direct_coinduction : basic_goal reaches.
+intros.
+repeat (eapply step;[econstructor (reflexivity || find_map_entry)|]);apply done.
+repeat split;equate_maps.
+Qed.
+
+(* Using tactics for kstep, kequiv *)
+Lemma basic_tacs : basic_goal reaches.
+intros.
+repeat (eapply step;[kstep_tac|]);apply done;kequiv_tac.
+Qed.
+
+Ltac steps_run := repeat (eapply step;[kstep_tac|]);apply done;kequiv_tac.
+
+(* Now using derived rules *)
+
+(* Try to either finish immediately or take a step at a stepF goal *)
+Ltac first_step := (apply DoneF;kequiv_tac) || (eapply StepF;[kstep_tac|]).
+Ltac by_rules rules := let H :=
+  fresh in assert (sound rules) as H;[apply trans_sound;destruct 1;first_step|intros;apply H;constructor].
+
+Inductive basic_rule : RRel := BasicGoal : basic_goal basic_rule.
+
+Lemma derived_rules : basic_goal reaches.
+by_rules basic_rule.
+repeat (eapply tstep;[kstep_tac|]);apply tdone;kequiv_tac.
+Qed.
+
+(* Make a basic run tactic *)
+Ltac tstep_tac := eapply tstep;[kstep_tac|].
+Ltac tfinish_tac := solve[apply tdone;kequiv_tac].
+
+Ltac trun_basic := repeat tstep_tac;try tfinish_tac.
+
+Lemma trun_basic_test : basic_goal reaches.
+by_rules basic_rule;trun_basic.
+Qed.
+
+Notation heap_goal rel :=
+  (forall p env, rel (KCfg (kra (HAssign "x" (EPlus (ELoad "x") 1%Z)) nil)
+              (env :* "x" |-> p) (p |-> 12%Z) mapEmpty)
+        (kequiv (KCfg nil (env :* "x" |-> p) (p |-> 13%Z) mapEmpty))).
+
+Inductive heap_rule : RRel := HeapGoal : heap_goal heap_rule.
+(* Now an example program that has a heap *)
+Lemma heap_test : heap_goal reaches.
+Proof.
+by_rules heap_rule;trun_basic.
+Qed.
+
+(* Slightly more compilicated example, needing to split. *)
 Definition step (state event : Z) :=
-  match event, state with
+  match state, event with
     | Z0, Z0 => 1
     | _, _ => 0
   end.
+Lemma step_ZZ : forall s e, s = 0 -> e = 0 -> step s e = 1.
+intros;subst;reflexivity. Qed.
+Lemma step_N1 : forall s e, s <> 0 -> step s e = 0.
+intros;destruct s;simpl;congruence. Qed.
+Lemma step_N2 : forall s e, e <> 0 -> step s e = 0.
+intros;destruct s;destruct e;simpl;congruence. Qed.
+Create HintDb step_simpl discriminated.
+Hint Rewrite step_ZZ step_N1 step_N2 using assumption: step_simpl.
 
-Lemma update_function : forall state addr event,
-  steps (KCfg (kra (SIf
+Notation split_goal rel := (forall state addr event,
+  rel (KCfg (kra (SIf
                  (BAnd (BEq (ELoad "state") 0) (BEq "event" 0))
                  (HAssign "state" 1)
                  (HAssign "state" 0)) nil)
               ("event" |-> event :* "state" |-> addr) (addr |-> state) mapEmpty)
-        (KCfg nil
-              ("event" |-> event :* "state" |-> addr) (addr |-> (step state event)) mapEmpty).
+      (kequiv (KCfg nil
+              ("event" |-> event :* "state" |-> addr) (addr |-> (step state event)) mapEmpty))).
+Inductive split_rules : RRel := SplitGoal : split_goal split_rules.
+
+(* First split manually *)
+Lemma manual_split : split_goal reaches.
 Proof.
-intros.
-run;destruct state;destruct event;
-simpl;(congruence || reflexivity).
+by_rules split_rules;trun_basic.
+(* Gets stuck at split *)
+destruct state;trun_basic.
+destruct event;trun_basic.
 Qed. 
 Close Scope Z_scope.
 
-Lemma heap_test : forall p env,
-  steps (KCfg (kra (HAssign "x" (EPlus (ELoad "x") 1%Z)) nil)
-              (env :* "x" |-> p) (p |-> 12%Z) mapEmpty)
-        (KCfg nil (env :* "x" |-> p) (p |-> 13%Z) mapEmpty).
-Proof.
-intros.
-repeat (refine (more _ (@kequiv_refl _) _ _);[econstructor(reflexivity||find_map_entry)|]).
-finish.
-Qed.
+Ltac split_bool bexp :=
+  match bexp with
+    | negb ?bexp' => split_bool bexp'
+    | (?x <=? ?y)%Z => destruct (Z.leb_spec x y)
+    | (?x =? ?y)%Z  => destruct (Z.eqb_spec x y)
+  end.
+Ltac tsplit_if :=
+  cbv beta; match goal with
+      | [|- trans _ (KCfg (kra (KStmt (SIf (BCon ?test) _ _)) _) _ _ _) _] => split_bool test
+      | [|- trans _ (KCfg (kra (KBExp (BAnd (BCon ?test) _)) _) _ _ _) _] => split_bool test
+  end.
 
+Ltac trun_split finish_simpl := repeat (tstep_tac || tsplit_if);finish_simpl;try tfinish_tac.
+
+Lemma auto_split : split_goal reaches.
+Proof.
+by_rules split_rules;trun_split ltac:(autorewrite with step_simpl).
+Qed. 
+Close Scope Z_scope.
+
+(* List reverse *) 
 Definition listrev :=
   (SWhile (BNot (BEq 0%Z "p"))
-     (Seq (SAssign "next" (ELoad (EPlus "p" 1%Z)))
+     (Seq (SAssign "next" (ELoad (EPlus "p" 1%Z))) 
      (Seq (HAssign (EPlus "p" 1%Z) "q")
      (Seq (SAssign "q" "p")
           (SAssign "p" "next"))))).
 
+(* Representation predicate *)
 Fixpoint listrep (l : list Z) (p : Z) (m : Map Z Z) : Prop :=
   match l with
     | nil => p = 0%Z /\ m ~= mapEmpty
@@ -60,20 +170,20 @@ Fixpoint listrep (l : list Z) (p : Z) (m : Map Z Z) : Prop :=
          /\ listrep l' next m'
   end.
 
+(*
 Ltac same_eprefix H :=
   match goal with
       [ H : exists _ : ?A , _ |- exists _ : ?A , _ ] =>
       let x := fresh "x" in destruct H as [x H]; exists x
   end.
-  
+*)
+
 Lemma listrep_equiv : forall l p m m', m ~= m' -> listrep l p m -> listrep l p m'.
 destruct l;simpl; intuition.
-rewrite <- H; assumption.
-repeat same_eprefix H2.
-intuition.
-rewrite <- H; assumption.
+setoid_rewrite <- H; assumption.
 Qed.
 
+(* Test a concrete execution of list reverse *)
 Lemma rev_test : forall lenv,
   steps (KCfg (kra listrev nil)
               ("p" |-> 1 :* "q" |-> 0 :* "next" |-> 1)%Z
@@ -88,17 +198,8 @@ Lemma rev_test : forall lenv,
                5 |-> 14 :* 6 |-> 3)%Z
               lenv).
 Proof.
-intros;repeat step_rule;finish.
+intros;steps_run.
 Qed.
-
-(* For a generic statement about reverse, we would like
-   to have an existential about the address the reversed
-   list starts at, need a different sort of reaching
-   to let us put the existential where we like. *)
-
-CoInductive reaches (s : kcfg) (phi : kcfg -> Prop) : Prop :=
- | r_done : phi s -> reaches s phi
- | r_more : forall s', kstep s s' -> reaches s' phi -> reaches s phi.
 
 (* Brute force attempt to simplify all representation predicates *)
 Ltac simplify_listrep := repeat
@@ -112,6 +213,22 @@ Ltac simplify_listrep := repeat
         try (rewrite H in * |- *;clear H heap)
   end.
 
+(* Need to adjust tactics to stop at circularities, and maybe do something
+   about automatically cleaning up lists *)
+
+(* Idea 1: assume circularities have non-overlapping <k> in left-hand side,
+   so we can commit to the first that unifies and (fail 1) if we couldn't
+   satisfy it's hypotheses *)
+(* Idea 2: add into the run cycle a tactic that recognizes lookups on an
+   address registered with a representation predicate, and unfolds/splits to
+   make progress
+ *)
+(* Idea 3: probably folding can be handled by writing invariant rules with
+   folded conclusions, and then we only have to deal with it at the finish
+   while trying to validate that rule
+ *)
+
+(*
 Ltac stop_at_circ circ := (eapply circ; fail 1).
 (* add to find_map_entry a thing that unfolds/splits *)
 Ltac r_step := (eapply r_more;[solve[econstructor(reflexivity||find_map_entry)]|]).
@@ -163,39 +280,6 @@ simpl. split;[congruence|]. eexists;eexists;split;[|eassumption].
 equate_maps.
 Qed.
 
-Function evals n kcfg :=
-  match n with
-    | 0 => kcfg
-    | S n => 
-      match eval kcfg with
-      | Some kcfg' => evals n kcfg'
-      | None => kcfg
-     end
-  end.
-
-Lemma evals_sound :
-  forall n c1 c2,
-    kequiv (evals n c1) c2 -> steps c1 c2.
-Proof.
-induction n; simpl; intros c1 c2.
-apply done.
-pose proof (eval_sound c1).
-destruct (eval c1).
-intro.
-apply more with c1 k. reflexivity.
-assumption. apply IHn. assumption.
-apply done.
-Qed.
-
-Lemma eval_happy : forall env,
-  steps (KCfg (kra (SAssign "x" (EPlus "x" "y")) nil)
-            (env :* "x" |-> 12%Z :* "y" |-> 13%Z) mapEmpty mapEmpty)
-        (KCfg nil (env :* "x" |-> 25%Z :* "y" |-> 13%Z) mapEmpty mapEmpty).
-intros.
-repeat (refine (more _ (@kequiv_refl _) _ _);[econstructor (reflexivity || find_map_entry)|]);
-simpl Zplus; finish.
-Qed.
-
 (* Try "quote" on the env *)
 (* Use a mixed coinductive sequencing to use loop invariants? *)
 
@@ -215,60 +299,4 @@ CoFixpoint sum :
           ("i" |-> 0%Z :* "j" |-> z%Z :* erest) heap labels).
 intros; step_rule;run_circ sum.
 Qed.
-
-Lemma eval_happy' : forall env,
-  steps (KCfg (kra (SAssign "x" (EPlus "x" "y")) nil)
-            ("x" |-> 12%Z :* "y" |-> 13%Z :* env) mapEmpty mapEmpty)
-        (KCfg nil ("x" |-> 25%Z :* "y" |-> 13%Z :* env) mapEmpty mapEmpty).
-intros;
-repeat (refine (more _ (@kequiv_refl _) _ _);[match goal with [|- kstep ?l _] => eapply (eval_sound l) end|]);
-simpl Zplus; finish.
-Qed.
-
-Definition gcdProg : Map string Stmt :=
-  "gcd" |->
-        SIf (BLe "a" "b")
-          (SIf (BLe "b" "a")
-               (Jump "done")
-               (Seq (SAssign "b" (EMinus "b" "a"))
-                    (Jump "gcd")))
-          (Seq (SAssign "a" (EMinus "a" "b"))
-               (Jump "gcd")).
-Lemma label_eval : forall env,
-  steps (KCfg (kra (Jump "gcd") kdot)
-            ("a" |-> 12%Z :* "b" |-> 13%Z :* env) mapEmpty gcdProg)
-        (KCfg (kra (Jump "done") kdot)
-             ("a" |-> 1%Z :* "b" |-> 1%Z :* env) mapEmpty gcdProg).
-intros. apply evals_sound with 307; simpl; repeat split; reflexivity.
-Qed.
-
-(* Some performance tests *)
-Lemma loop_test:
-  steps (KCfg (kra (SWhile (BLe 0%Z "x")
-    (SAssign "x" (EPlus "x" (-1)%Z)))
-  nil) ("x" |-> 25%Z) mapEmpty mapEmpty)
-  (KCfg nil ("x" |-> (-1)%Z) mapEmpty mapEmpty).
-Proof.
-intros;
-repeat (refine (more _ (@kequiv_refl _) _ _);[econstructor (reflexivity || find_map_entry)|];instantiate;simpl Zplus);
-finish.
-Qed.
-
-Lemma loop_test':
-  steps (KCfg (kra (SWhile (BLe 0%Z "x")
-    (SAssign "x" (EPlus "x" (-1)%Z)))
-  nil) ("x" |-> 25%Z) mapEmpty mapEmpty)
-  (KCfg nil ("x" |-> (-1)%Z) mapEmpty mapEmpty).
-Proof.
-Ltac step_eval :=refine (more _ (@kequiv_refl _) _ _);[match goal with [|- kstep ?l _] => eapply (eval_sound l) end|].
-intros;repeat step_eval;simpl;finish.
-Qed.
-
-Lemma loop_test'':
-  steps (KCfg (kra (SWhile (BLe (ECon 0) (EVar "x"))
-    (SAssign "x" (EPlus (EVar "x") (ECon (-1)%Z))))
-  nil) ("x" |-> 25%Z) mapEmpty mapEmpty)
-  (KCfg nil ("x" |-> (-1)%Z) mapEmpty mapEmpty).
-Proof.
-intros;apply (evals_sound 1000);lazy;repeat (apply conj);[reflexivity|simpl;equate_maps ..].
-Qed.
+ *)
